src/compiler_generic/toy_example/document_generated/Design_generated_generated.thy
@@ -149,12 +149,20 @@ lemma perm_\<sigma>\<^sub>1 : "\<sigma>\<^sub>1 = (state.make ((Map.empty (oid2 
 by(simp)
 end
 
-(* 17 ************************************ 36 + 1 *)
+(* 17 ************************************ 36 + 2 *)
+definition "oid8 = 8"
+definition "inst_assoc8 = (\<lambda>oid_class to_from oid. ((case (deref_assocs_list ((to_from::oid list list \<Rightarrow> oid list \<times> oid list)) ((oid::oid)) ((drop ((((map_of_list ([]))) ((oid_class::oid))))))) of Nil \<Rightarrow> None
+    | l \<Rightarrow> (Some (l)))::oid list option))"
+
+(* 18 ************************************ 38 + 0 *)
+
+(* 19 ************************************ 38 + 1 *)
 locale state_\<sigma>\<^sub>1' =
 fixes "oid1" :: "nat"
 fixes "oid2" :: "nat"
 fixes "oid3" :: "nat"
-assumes distinct_oid: "(distinct ([oid1 , oid2 , oid3]))"
+fixes "oid8" :: "nat"
+assumes distinct_oid: "(distinct ([oid1 , oid2 , oid3 , oid8]))"
 fixes "X\<^sub>P\<^sub>e\<^sub>r\<^sub>s\<^sub>o\<^sub>n1\<^sub>P\<^sub>e\<^sub>r\<^sub>s\<^sub>o\<^sub>n" :: "ty\<^sub>P\<^sub>e\<^sub>r\<^sub>s\<^sub>o\<^sub>n"
 fixes "X\<^sub>P\<^sub>e\<^sub>r\<^sub>s\<^sub>o\<^sub>n1" :: "\<cdot>Person"
 assumes X\<^sub>P\<^sub>e\<^sub>r\<^sub>s\<^sub>o\<^sub>n1_def: "X\<^sub>P\<^sub>e\<^sub>r\<^sub>s\<^sub>o\<^sub>n1 = (\<lambda>_. \<lfloor>\<lfloor>X\<^sub>P\<^sub>e\<^sub>r\<^sub>s\<^sub>o\<^sub>n1\<^sub>P\<^sub>e\<^sub>r\<^sub>s\<^sub>o\<^sub>n\<rfloor>\<rfloor>)"
@@ -164,18 +172,24 @@ assumes X\<^sub>P\<^sub>e\<^sub>r\<^sub>s\<^sub>o\<^sub>n2_def: "X\<^sub>P\<^sub
 fixes "X\<^sub>P\<^sub>e\<^sub>r\<^sub>s\<^sub>o\<^sub>n3\<^sub>P\<^sub>e\<^sub>r\<^sub>s\<^sub>o\<^sub>n" :: "ty\<^sub>P\<^sub>e\<^sub>r\<^sub>s\<^sub>o\<^sub>n"
 fixes "X\<^sub>P\<^sub>e\<^sub>r\<^sub>s\<^sub>o\<^sub>n3" :: "\<cdot>Person"
 assumes X\<^sub>P\<^sub>e\<^sub>r\<^sub>s\<^sub>o\<^sub>n3_def: "X\<^sub>P\<^sub>e\<^sub>r\<^sub>s\<^sub>o\<^sub>n3 = (\<lambda>_. \<lfloor>\<lfloor>X\<^sub>P\<^sub>e\<^sub>r\<^sub>s\<^sub>o\<^sub>n3\<^sub>P\<^sub>e\<^sub>r\<^sub>s\<^sub>o\<^sub>n\<rfloor>\<rfloor>)"
+fixes "X\<^sub>P\<^sub>e\<^sub>r\<^sub>s\<^sub>o\<^sub>n4\<^sub>P\<^sub>e\<^sub>r\<^sub>s\<^sub>o\<^sub>n" :: "ty\<^sub>P\<^sub>e\<^sub>r\<^sub>s\<^sub>o\<^sub>n"
+fixes "X\<^sub>P\<^sub>e\<^sub>r\<^sub>s\<^sub>o\<^sub>n4" :: "\<cdot>Person"
+assumes X\<^sub>P\<^sub>e\<^sub>r\<^sub>s\<^sub>o\<^sub>n4_def: "X\<^sub>P\<^sub>e\<^sub>r\<^sub>s\<^sub>o\<^sub>n4 = (\<lambda>_. \<lfloor>\<lfloor>X\<^sub>P\<^sub>e\<^sub>r\<^sub>s\<^sub>o\<^sub>n4\<^sub>P\<^sub>e\<^sub>r\<^sub>s\<^sub>o\<^sub>n\<rfloor>\<rfloor>)"
 begin
-definition "\<sigma>\<^sub>1' = (state.make ((Map.empty (oid1 \<mapsto> (in\<^sub>P\<^sub>e\<^sub>r\<^sub>s\<^sub>o\<^sub>n (X\<^sub>P\<^sub>e\<^sub>r\<^sub>s\<^sub>o\<^sub>n1\<^sub>P\<^sub>e\<^sub>r\<^sub>s\<^sub>o\<^sub>n))) (oid2 \<mapsto> (in\<^sub>P\<^sub>e\<^sub>r\<^sub>s\<^sub>o\<^sub>n (X\<^sub>P\<^sub>e\<^sub>r\<^sub>s\<^sub>o\<^sub>n2\<^sub>P\<^sub>e\<^sub>r\<^sub>s\<^sub>o\<^sub>n))) (oid3 \<mapsto> (in\<^sub>P\<^sub>e\<^sub>r\<^sub>s\<^sub>o\<^sub>n (X\<^sub>P\<^sub>e\<^sub>r\<^sub>s\<^sub>o\<^sub>n3\<^sub>P\<^sub>e\<^sub>r\<^sub>s\<^sub>o\<^sub>n))))) ((map_of_list ([(oid\<^sub>P\<^sub>e\<^sub>r\<^sub>s\<^sub>o\<^sub>n_0___boss , (List.map ((\<lambda>(x , y). [x , y]) o switch\<^sub>2_01) ([[[oid1] , [oid2]]])))]))))"
+definition "\<sigma>\<^sub>1' = (state.make ((Map.empty (oid1 \<mapsto> (in\<^sub>P\<^sub>e\<^sub>r\<^sub>s\<^sub>o\<^sub>n (X\<^sub>P\<^sub>e\<^sub>r\<^sub>s\<^sub>o\<^sub>n1\<^sub>P\<^sub>e\<^sub>r\<^sub>s\<^sub>o\<^sub>n))) (oid2 \<mapsto> (in\<^sub>P\<^sub>e\<^sub>r\<^sub>s\<^sub>o\<^sub>n (X\<^sub>P\<^sub>e\<^sub>r\<^sub>s\<^sub>o\<^sub>n2\<^sub>P\<^sub>e\<^sub>r\<^sub>s\<^sub>o\<^sub>n))) (oid3 \<mapsto> (in\<^sub>P\<^sub>e\<^sub>r\<^sub>s\<^sub>o\<^sub>n (X\<^sub>P\<^sub>e\<^sub>r\<^sub>s\<^sub>o\<^sub>n3\<^sub>P\<^sub>e\<^sub>r\<^sub>s\<^sub>o\<^sub>n))) (oid8 \<mapsto> (in\<^sub>P\<^sub>e\<^sub>r\<^sub>s\<^sub>o\<^sub>n (X\<^sub>P\<^sub>e\<^sub>r\<^sub>s\<^sub>o\<^sub>n4\<^sub>P\<^sub>e\<^sub>r\<^sub>s\<^sub>o\<^sub>n))))) ((map_of_list ([(oid\<^sub>P\<^sub>e\<^sub>r\<^sub>s\<^sub>o\<^sub>n_0___boss , (List.map ((\<lambda>(x , y). [x , y]) o switch\<^sub>2_01) ([[[oid1] , [oid2]]])))]))))"
 
-lemma perm_\<sigma>\<^sub>1' : "\<sigma>\<^sub>1' = (state.make ((Map.empty (oid3 \<mapsto> (in\<^sub>P\<^sub>e\<^sub>r\<^sub>s\<^sub>o\<^sub>n (X\<^sub>P\<^sub>e\<^sub>r\<^sub>s\<^sub>o\<^sub>n3\<^sub>P\<^sub>e\<^sub>r\<^sub>s\<^sub>o\<^sub>n))) (oid2 \<mapsto> (in\<^sub>P\<^sub>e\<^sub>r\<^sub>s\<^sub>o\<^sub>n (X\<^sub>P\<^sub>e\<^sub>r\<^sub>s\<^sub>o\<^sub>n2\<^sub>P\<^sub>e\<^sub>r\<^sub>s\<^sub>o\<^sub>n))) (oid1 \<mapsto> (in\<^sub>P\<^sub>e\<^sub>r\<^sub>s\<^sub>o\<^sub>n (X\<^sub>P\<^sub>e\<^sub>r\<^sub>s\<^sub>o\<^sub>n1\<^sub>P\<^sub>e\<^sub>r\<^sub>s\<^sub>o\<^sub>n))))) ((assocs (\<sigma>\<^sub>1'))))"
+lemma perm_\<sigma>\<^sub>1' : "\<sigma>\<^sub>1' = (state.make ((Map.empty (oid8 \<mapsto> (in\<^sub>P\<^sub>e\<^sub>r\<^sub>s\<^sub>o\<^sub>n (X\<^sub>P\<^sub>e\<^sub>r\<^sub>s\<^sub>o\<^sub>n4\<^sub>P\<^sub>e\<^sub>r\<^sub>s\<^sub>o\<^sub>n))) (oid3 \<mapsto> (in\<^sub>P\<^sub>e\<^sub>r\<^sub>s\<^sub>o\<^sub>n (X\<^sub>P\<^sub>e\<^sub>r\<^sub>s\<^sub>o\<^sub>n3\<^sub>P\<^sub>e\<^sub>r\<^sub>s\<^sub>o\<^sub>n))) (oid2 \<mapsto> (in\<^sub>P\<^sub>e\<^sub>r\<^sub>s\<^sub>o\<^sub>n (X\<^sub>P\<^sub>e\<^sub>r\<^sub>s\<^sub>o\<^sub>n2\<^sub>P\<^sub>e\<^sub>r\<^sub>s\<^sub>o\<^sub>n))) (oid1 \<mapsto> (in\<^sub>P\<^sub>e\<^sub>r\<^sub>s\<^sub>o\<^sub>n (X\<^sub>P\<^sub>e\<^sub>r\<^sub>s\<^sub>o\<^sub>n1\<^sub>P\<^sub>e\<^sub>r\<^sub>s\<^sub>o\<^sub>n))))) ((assocs (\<sigma>\<^sub>1'))))"
   apply(simp add: \<sigma>\<^sub>1'_def)
   apply(subst (1) fun_upd_twist, metis distinct_oid distinct_length_2_or_more)
+  apply(subst (2) fun_upd_twist, metis distinct_oid distinct_length_2_or_more)
+  apply(subst (1) fun_upd_twist, metis distinct_oid distinct_length_2_or_more)
+  apply(subst (3) fun_upd_twist, metis distinct_oid distinct_length_2_or_more)
   apply(subst (2) fun_upd_twist, metis distinct_oid distinct_length_2_or_more)
   apply(subst (1) fun_upd_twist, metis distinct_oid distinct_length_2_or_more)
 by(simp)
 end
 
-(* 18 ************************************ 37 + 1 *)
+(* 20 ************************************ 39 + 1 *)
 locale pre_post_\<sigma>\<^sub>1_\<sigma>\<^sub>1' =
 fixes "oid1" :: "nat"
 fixes "oid2" :: "nat"
@@ -184,7 +198,8 @@ fixes "oid4" :: "nat"
 fixes "oid5" :: "nat"
 fixes "oid6" :: "nat"
 fixes "oid7" :: "nat"
-assumes distinct_oid: "(distinct ([oid1 , oid2 , oid3 , oid4 , oid5 , oid6 , oid7]))"
+fixes "oid8" :: "nat"
+assumes distinct_oid: "(distinct ([oid1 , oid2 , oid3 , oid4 , oid5 , oid6 , oid7 , oid8]))"
 fixes "X\<^sub>P\<^sub>e\<^sub>r\<^sub>s\<^sub>o\<^sub>n1\<^sub>P\<^sub>e\<^sub>r\<^sub>s\<^sub>o\<^sub>n" :: "ty\<^sub>P\<^sub>e\<^sub>r\<^sub>s\<^sub>o\<^sub>n"
 fixes "X\<^sub>P\<^sub>e\<^sub>r\<^sub>s\<^sub>o\<^sub>n1" :: "\<cdot>Person"
 assumes X\<^sub>P\<^sub>e\<^sub>r\<^sub>s\<^sub>o\<^sub>n1_def: "X\<^sub>P\<^sub>e\<^sub>r\<^sub>s\<^sub>o\<^sub>n1 = (\<lambda>_. \<lfloor>\<lfloor>X\<^sub>P\<^sub>e\<^sub>r\<^sub>s\<^sub>o\<^sub>n1\<^sub>P\<^sub>e\<^sub>r\<^sub>s\<^sub>o\<^sub>n\<rfloor>\<rfloor>)"
@@ -206,15 +221,18 @@ assumes \<sigma>\<^sub>1_object2_def: "\<sigma>\<^sub>1_object2 = (\<lambda>_. \
 fixes "\<sigma>\<^sub>1_object4\<^sub>P\<^sub>e\<^sub>r\<^sub>s\<^sub>o\<^sub>n" :: "ty\<^sub>P\<^sub>e\<^sub>r\<^sub>s\<^sub>o\<^sub>n"
 fixes "\<sigma>\<^sub>1_object4" :: "\<cdot>Person"
 assumes \<sigma>\<^sub>1_object4_def: "\<sigma>\<^sub>1_object4 = (\<lambda>_. \<lfloor>\<lfloor>\<sigma>\<^sub>1_object4\<^sub>P\<^sub>e\<^sub>r\<^sub>s\<^sub>o\<^sub>n\<rfloor>\<rfloor>)"
+fixes "X\<^sub>P\<^sub>e\<^sub>r\<^sub>s\<^sub>o\<^sub>n4\<^sub>P\<^sub>e\<^sub>r\<^sub>s\<^sub>o\<^sub>n" :: "ty\<^sub>P\<^sub>e\<^sub>r\<^sub>s\<^sub>o\<^sub>n"
+fixes "X\<^sub>P\<^sub>e\<^sub>r\<^sub>s\<^sub>o\<^sub>n4" :: "\<cdot>Person"
+assumes X\<^sub>P\<^sub>e\<^sub>r\<^sub>s\<^sub>o\<^sub>n4_def: "X\<^sub>P\<^sub>e\<^sub>r\<^sub>s\<^sub>o\<^sub>n4 = (\<lambda>_. \<lfloor>\<lfloor>X\<^sub>P\<^sub>e\<^sub>r\<^sub>s\<^sub>o\<^sub>n4\<^sub>P\<^sub>e\<^sub>r\<^sub>s\<^sub>o\<^sub>n\<rfloor>\<rfloor>)"
 
 assumes \<sigma>\<^sub>1: "(state_\<sigma>\<^sub>1 (oid4) (oid5) (oid6) (oid1) (oid7) (oid2) (\<sigma>\<^sub>1_object0\<^sub>P\<^sub>e\<^sub>r\<^sub>s\<^sub>o\<^sub>n) (\<sigma>\<^sub>1_object0) (\<sigma>\<^sub>1_object1\<^sub>P\<^sub>e\<^sub>r\<^sub>s\<^sub>o\<^sub>n) (\<sigma>\<^sub>1_object1) (\<sigma>\<^sub>1_object2\<^sub>P\<^sub>e\<^sub>r\<^sub>s\<^sub>o\<^sub>n) (\<sigma>\<^sub>1_object2) (X\<^sub>P\<^sub>e\<^sub>r\<^sub>s\<^sub>o\<^sub>n1\<^sub>P\<^sub>e\<^sub>r\<^sub>s\<^sub>o\<^sub>n) (X\<^sub>P\<^sub>e\<^sub>r\<^sub>s\<^sub>o\<^sub>n1) (\<sigma>\<^sub>1_object4\<^sub>P\<^sub>e\<^sub>r\<^sub>s\<^sub>o\<^sub>n) (\<sigma>\<^sub>1_object4) (X\<^sub>P\<^sub>e\<^sub>r\<^sub>s\<^sub>o\<^sub>n2\<^sub>P\<^sub>e\<^sub>r\<^sub>s\<^sub>o\<^sub>n) (X\<^sub>P\<^sub>e\<^sub>r\<^sub>s\<^sub>o\<^sub>n2))"
 
-assumes \<sigma>\<^sub>1': "(state_\<sigma>\<^sub>1' (oid1) (oid2) (oid3) (X\<^sub>P\<^sub>e\<^sub>r\<^sub>s\<^sub>o\<^sub>n1\<^sub>P\<^sub>e\<^sub>r\<^sub>s\<^sub>o\<^sub>n) (X\<^sub>P\<^sub>e\<^sub>r\<^sub>s\<^sub>o\<^sub>n1) (X\<^sub>P\<^sub>e\<^sub>r\<^sub>s\<^sub>o\<^sub>n2\<^sub>P\<^sub>e\<^sub>r\<^sub>s\<^sub>o\<^sub>n) (X\<^sub>P\<^sub>e\<^sub>r\<^sub>s\<^sub>o\<^sub>n2) (X\<^sub>P\<^sub>e\<^sub>r\<^sub>s\<^sub>o\<^sub>n3\<^sub>P\<^sub>e\<^sub>r\<^sub>s\<^sub>o\<^sub>n) (X\<^sub>P\<^sub>e\<^sub>r\<^sub>s\<^sub>o\<^sub>n3))"
+assumes \<sigma>\<^sub>1': "(state_\<sigma>\<^sub>1' (oid1) (oid2) (oid3) (oid8) (X\<^sub>P\<^sub>e\<^sub>r\<^sub>s\<^sub>o\<^sub>n1\<^sub>P\<^sub>e\<^sub>r\<^sub>s\<^sub>o\<^sub>n) (X\<^sub>P\<^sub>e\<^sub>r\<^sub>s\<^sub>o\<^sub>n1) (X\<^sub>P\<^sub>e\<^sub>r\<^sub>s\<^sub>o\<^sub>n2\<^sub>P\<^sub>e\<^sub>r\<^sub>s\<^sub>o\<^sub>n) (X\<^sub>P\<^sub>e\<^sub>r\<^sub>s\<^sub>o\<^sub>n2) (X\<^sub>P\<^sub>e\<^sub>r\<^sub>s\<^sub>o\<^sub>n3\<^sub>P\<^sub>e\<^sub>r\<^sub>s\<^sub>o\<^sub>n) (X\<^sub>P\<^sub>e\<^sub>r\<^sub>s\<^sub>o\<^sub>n3) (X\<^sub>P\<^sub>e\<^sub>r\<^sub>s\<^sub>o\<^sub>n4\<^sub>P\<^sub>e\<^sub>r\<^sub>s\<^sub>o\<^sub>n) (X\<^sub>P\<^sub>e\<^sub>r\<^sub>s\<^sub>o\<^sub>n4))"
 begin
 interpretation state_\<sigma>\<^sub>1: state_\<sigma>\<^sub>1 "oid4" "oid5" "oid6" "oid1" "oid7" "oid2" "\<sigma>\<^sub>1_object0\<^sub>P\<^sub>e\<^sub>r\<^sub>s\<^sub>o\<^sub>n" "\<sigma>\<^sub>1_object0" "\<sigma>\<^sub>1_object1\<^sub>P\<^sub>e\<^sub>r\<^sub>s\<^sub>o\<^sub>n" "\<sigma>\<^sub>1_object1" "\<sigma>\<^sub>1_object2\<^sub>P\<^sub>e\<^sub>r\<^sub>s\<^sub>o\<^sub>n" "\<sigma>\<^sub>1_object2" "X\<^sub>P\<^sub>e\<^sub>r\<^sub>s\<^sub>o\<^sub>n1\<^sub>P\<^sub>e\<^sub>r\<^sub>s\<^sub>o\<^sub>n" "X\<^sub>P\<^sub>e\<^sub>r\<^sub>s\<^sub>o\<^sub>n1" "\<sigma>\<^sub>1_object4\<^sub>P\<^sub>e\<^sub>r\<^sub>s\<^sub>o\<^sub>n" "\<sigma>\<^sub>1_object4" "X\<^sub>P\<^sub>e\<^sub>r\<^sub>s\<^sub>o\<^sub>n2\<^sub>P\<^sub>e\<^sub>r\<^sub>s\<^sub>o\<^sub>n" "X\<^sub>P\<^sub>e\<^sub>r\<^sub>s\<^sub>o\<^sub>n2"
 by(rule \<sigma>\<^sub>1)
 
-interpretation state_\<sigma>\<^sub>1': state_\<sigma>\<^sub>1' "oid1" "oid2" "oid3" "X\<^sub>P\<^sub>e\<^sub>r\<^sub>s\<^sub>o\<^sub>n1\<^sub>P\<^sub>e\<^sub>r\<^sub>s\<^sub>o\<^sub>n" "X\<^sub>P\<^sub>e\<^sub>r\<^sub>s\<^sub>o\<^sub>n1" "X\<^sub>P\<^sub>e\<^sub>r\<^sub>s\<^sub>o\<^sub>n2\<^sub>P\<^sub>e\<^sub>r\<^sub>s\<^sub>o\<^sub>n" "X\<^sub>P\<^sub>e\<^sub>r\<^sub>s\<^sub>o\<^sub>n2" "X\<^sub>P\<^sub>e\<^sub>r\<^sub>s\<^sub>o\<^sub>n3\<^sub>P\<^sub>e\<^sub>r\<^sub>s\<^sub>o\<^sub>n" "X\<^sub>P\<^sub>e\<^sub>r\<^sub>s\<^sub>o\<^sub>n3"
+interpretation state_\<sigma>\<^sub>1': state_\<sigma>\<^sub>1' "oid1" "oid2" "oid3" "oid8" "X\<^sub>P\<^sub>e\<^sub>r\<^sub>s\<^sub>o\<^sub>n1\<^sub>P\<^sub>e\<^sub>r\<^sub>s\<^sub>o\<^sub>n" "X\<^sub>P\<^sub>e\<^sub>r\<^sub>s\<^sub>o\<^sub>n1" "X\<^sub>P\<^sub>e\<^sub>r\<^sub>s\<^sub>o\<^sub>n2\<^sub>P\<^sub>e\<^sub>r\<^sub>s\<^sub>o\<^sub>n" "X\<^sub>P\<^sub>e\<^sub>r\<^sub>s\<^sub>o\<^sub>n2" "X\<^sub>P\<^sub>e\<^sub>r\<^sub>s\<^sub>o\<^sub>n3\<^sub>P\<^sub>e\<^sub>r\<^sub>s\<^sub>o\<^sub>n" "X\<^sub>P\<^sub>e\<^sub>r\<^sub>s\<^sub>o\<^sub>n3" "X\<^sub>P\<^sub>e\<^sub>r\<^sub>s\<^sub>o\<^sub>n4\<^sub>P\<^sub>e\<^sub>r\<^sub>s\<^sub>o\<^sub>n" "X\<^sub>P\<^sub>e\<^sub>r\<^sub>s\<^sub>o\<^sub>n4"
 by(rule \<sigma>\<^sub>1')
 end
 
